src/program_proof/mpaxos/applyasfollower_proof.v
@@ -19,7 +19,7 @@ Lemma wp_singleClerk__applyAsFollower ck γ γsrv σ args_ptr args :
         "#HP" ∷ □ Pwf args.(applyAsFollowerArgs.state) ∗
         "%Hσ_index" ∷ ⌜ length σ = (int.nat args.(applyAsFollowerArgs.nextIndex))%nat ⌝ ∗
         "%Hghost_op_σ" ∷ ⌜ last σ.*1 = Some args.(applyAsFollowerArgs.state) ⌝ ∗
-        "#Hprop" ∷ is_proposal γ args.(applyAsFollowerArgs.epoch) σ
+        "#Hprop" ∷ is_proposal γ.(s_mp) args.(applyAsFollowerArgs.epoch) σ
   }}}
     singleClerk__applyAsFollower #ck #args_ptr
   {{{
@@ -45,12 +45,10 @@ Proof.
   iDestruct (own_slice_to_small with "Hsl") as "Hsl".
   iApply (wp_frame_wand with "[HΦ]").
   { iNamedAccu. }
+  unfold is_mpaxos_host.
+  iNamed "Hsrv".
   wp_apply (wp_ReconnectingClient__Call2 with "Hcl_rpc [] Hsl Hrep").
-  {
-    unfold is_mpaxos_host.
-    iNamed "Hsrv".
-    iFrame "#".
-  }
+  { iFrame "#". }
   { (* Successful RPC *)
     iModIntro.
     iNext.
